Mbse.lean
@@ -37,7 +37,13 @@ import Mbse.BlockerAudit
 import Mbse.SynthesisPipeline
 import Mbse.PhiDecode
 import Mbse.HomWitnessConstruction
+import Mbse.HomSearch
+import Mbse.PhiChecker
 import Mbse.LivenessFragment
+import Mbse.DynamicsLivenessExplore
+import Mbse.DynamicsLivenessUResponse
+import Mbse.DirectLivenessFragment
+import Mbse.BoundedUnrolling
 import Mbse.LTLTactics
 import Mbse.BiImplicationFailures
 import Mbse.TracePropertyLayer
@@ -48,3 +54,5 @@ import Mbse.InverseSynthesis
 import Mbse.PaperClaimLinkage
 import Mbse.ClassicalAssertionalBridge
 import Mbse.WymoreExercises
+import Mbse.AssertionalFC
+import Mbse.Examples
