Makefile
@@ -7,3 +7,6 @@ check: build check-no-sorry
 
 check-no-sorry:
 	./scripts/check_no_sorry.sh
+
+report:
+	lake exe mbse
